books/countereg-gen/acl2s-parameter.lisp
@@ -1,7 +1,11 @@
+#|$ACL2s-Preamble$;
+(ld ;; Newline to fool ACL2/cert.pl dependency scanner
+ "portcullis.lsp")
+(acl2::begin-book t :ttags :all);$ACL2s-Preamble$|#
 
 (in-package "ACL2")
 (include-book "utilities")
-(include-book "xdoc/top" :dir :system)
+
 
 ;;; Keep the following defconst synced with all the acl2s parameters
 (defconst *acl2s-parameters* '(num-trials
@@ -20,14 +24,12 @@
 ;All user-defined parameters are stored here
 (table acl2s-defaults-table)
 
-
+(defrec acl2s-param-info% (value guard setter) NIL)
 
 (defmacro add-acl2s-parameter (name default
                                     &key 
                                     (setter 'nil)
-                                    (parents  'nil)
-                                    (short 'nil)
-                                    (long 'nil)
+                                    (doc-string 'nil)
                                     (guard 't))
   "Add a new user-defined parameter.
    Put it in the acl2s-defaults-table as a key,
@@ -41,19 +43,12 @@ embedded event form, this this is called from inside an make-event.
 You have to see the code in acl2s-defaults to understand whats going
 on with getter and setter, the situation is assymmetric and I am
 being lazy about documentation.
-:parents, :short and :long is used to specify the xdoc data. "
+:doc-string is a string that is used to specify the defdoc. 
+For internal flags dont use a doc-string"
   
   (b* (((unless (symbolp name))
         (er hard 'add-acl2s-parameter
             "Name must be a symbol, but is ~x0." name))
-#|
-       ((unless (and (acl2::good-map xdoc)
-                     (symbol-listp (mget :parents xdoc))
-                     (stringp (mget :short xdoc))
-                     (stringp (mget :long xdoc))))
-        (er hard 'add-acl2s-parameter 
-            ":xdoc must be a xdoc datatype, but is ~x0." xdoc))
-            |#
        ((unless (allp guard))
         (er hard 'add-acl2s-parameter 
             ":guard must be a term, but is ~x0." guard))
@@ -62,109 +57,146 @@ being lazy about documentation.
     `(progn 
        (table acl2s-defaults-table 
               ',name
-              ',(c nil :guard guard ;store guard too
-                  :value default
-                  :setter setter)
+              ',(acl2::make acl2s-param-info%
+                 :guard guard ;store guard too
+                 :value default
+                 :setter setter)
               :put)
-       (defxdoc ,name
-         :parents ,parents
-         :short ,short
-         :long ,long))))
+       ,@(and doc-string
+              `((defdoc ,name ,doc-string))))))
 
 
   
+
+
+(defdoc ACL2::TESTING
+  ":Doc-Section ACL2::TESTING
+  
+  A counterexample generation framework for ACL2 ~/
+                                 
+  Test formulas before and during a proof attempt, to find
+  counterexamples and witnesses potentially saving time and
+  effort and providing more intuition into the conjecture under
+  scrutiny.  The testing framework is tightly coupled with the
+  data definition (See ~ilc[DATA-DEFINITIONS]) framework.
+  
+  ~t[test?] guarantees printing counterexamples in
+  terms of the top goals variables. See ~ilc[test?]
+  for more details and examples.
+  
+  The framework can be configured via a bunch of parameters
+  whose documention you will find below. In particular, see
+  ~ilc[num-trials], ~ilc[verbosity-level], ~ilc[testing-enabled].~/ 
+  
+  To understand more about how testing works,
+  please refer to the following paper
+  ~url[http://www.ccs.neu.edu/home/harshrc/ITaITP.pdf]
+  ")
+
+
 (add-acl2s-parameter 
  num-trials 1000
- :parents (ACL2::TESTING)
- :short "Max number of tries to find counterexamples"
- :long 
-    "Maximum number of tries (attempts) to construct 
+ :doc-string 
+ ":Doc-Section ACL2::TESTING
+  
+  Max number of tries to find counterexamples~/~/
+
+  Maximum number of tries (attempts) to construct 
   counterexamples and witnesses.
   By default this parameter is set to 1000. Can be set to
-  any natural number <tt>n</tt>. If set to 0, it has the same
-  effect as setting testing-enabled parameter to <tt>nil</tt>.
-  <code>
+  any natural number ~t[n]. If set to 0, it has the same
+  effect as setting testing-enabled parameter to ~t[nil].
+  ~bv[]
    Usage:
    (acl2s-defaults :set num-trials 1000)
    (acl2s-defaults :get num-trials)
-   :xdoc num-trials
-  </code>"
+   :doc num-trials
+   ~ev[]"
  :guard (and (natp value) 
              (< value 1000000000)))
 
 (add-acl2s-parameter 
  verbosity-level 1
- :parents (ACL2::TESTING)
- :short "Control verbosity of Testing"
- :long "Control amount of output printed by random-testing
+ :doc-string 
+ ":Doc-Section ACL2::TESTING
+  
+ Control verbosity of Testing~/~/
+
+ Control amount of output printed by random-testing
    Currently 3 verbosity levels are implemented:
    0 - All testing output is turned off
-   1 - Normal verbosity levels (default)
+   1 - Normal verbosity level (default)
    2 - More verbose.
    3 - For Debug by normal users
    4 and above - System level debug by developers
-  <code>
+  ~bv[]
     Usage:
     (acl2s-defaults :set verbosity-level 1)
     (acl2s-defaults :get verbosity-level)
-    :xdoc verbosity-level
-   </code>"
+    :doc verbosity-level
+  ~ev[]"
  :guard (natp value))
 
 
 (add-acl2s-parameter 
   num-counterexamples 3
- :parents (ACL2::TESTING)
- :short "Number of Counterexamples to be shown"
- :long "Set the number of counterexamples desired to be shown~/
+ :doc-string 
+ ":Doc-Section ACL2::TESTING
+ 
+  Number of Counterexamples to be shown~/~/
+ 
+  Set the number of counterexamples desired to be shown
   By default this parameter is set to 3. Can be set to
-  any natural number <tt>n</tt>. Setting this number to 0 implies
+  any natural number n. Setting this number to 0 implies
   the user is not interested in seeing counterexamples, and
   thus none will be printed in the testing output.
   
-  <code>
+  ~bv[]
   Usage:
   (acl2s-defaults :set num-counterexamples 3)
   (acl2s-defaults :get num-counterexamples)
-  :xdoc num-counterexamples
-  </code>"
+  :doc num-counterexamples
+  ~ev[]"
    :guard (natp value))
 
 
 (add-acl2s-parameter 
   num-witnesses 3
- :parents (ACL2::TESTING)
- :short "Number of Witnesses to be shown"
- :long "Set the number of witnesses desired to be shown~/
+ :doc-string 
+ ":Doc-Section ACL2::TESTING
+  
+  Number of Witnesses to be shown~/~/
+  
+  Set the number of witnesses desired to be shown
   By default this parameter is set to 3. Can be set to
-  any natural number <tt>n</tt>. Setting this number to 0 implies
+  any natural number. Setting this number to 0 implies
   the user is not interested in seeing witnesses, and
   thus none will be printed in the testing output.
   
-  <code>
+  ~bv[]
   Usage:
   (acl2s-defaults :set num-witnesses 3)
   (acl2s-defaults :get num-witnesses)
-  :xdoc num-witnesses
-  </code>"
+  :doc num-witnesses
+  ~ev[]"
    :guard (natp value))
 
 ;DEPRECATED
 ;; (add-acl2s-parameter 
 ;;  show-top-level-counterexample t
-;;  :parents (ACL2::TESTING)
-;;  :short "Show Counterexamples to the top-level <i>goal</i>" 
-;;  :long "Show Counterexamples to the top-level <i>goal</i>
+;;  :doc-string ":Doc-Section ACL2::TESTING
+;;  Show Counterexamples to the top-level <i>goal</i>" 
+;;  Show Counterexamples to the top-level <i>goal</i>
 ;;    instead of to the <i>subgoals</i>.
 ;;    By default this parameter is set to <tt>t</tt>. 
 ;;    If set to <tt>nil</tt>, then counterexamples are simply
 ;;    instances falsifying the respective subgoals.
-;;    <code>
+;;    ~bv[]
 ;;    Usage:
 ;;    (acl2s-defaults :set show-top-level-counterexample t)
 ;;    (acl2s-defaults :get show-top-level-counterexample)
-;;    :xdoc show-top-level-counterexample 
-;;    </code>
+;;    :doc show-top-level-counterexample 
+;;    ~ev[]
 ;;    "
 ;;  :guard (booleanp value))
 
@@ -203,47 +235,53 @@ being lazy about documentation.
 
 (add-acl2s-parameter 
  search-strategy :simple
- :parents (ACL2::TESTING)
- :short "Specify the search strategy to be used" 
- :long "Specify which of the following strategies to
+ :doc-string 
+ ":Doc-Section ACL2::TESTING
+  
+  Specify the search strategy to be used ~/~/
+ 
+  Specify which of the following strategies to
   use for instantiating free variables of the conjecture
-  under test: <tt>:simple</tt> or <tt>:incremental</tt>
-  or <tt>:hybrid</tt>.
-  <tt>:incremental</tt> uses a dpll-like algorithm to search
-for counterexamples.
+  under test: ~t[:simple] or  ~t[:incremental]
+  or  ~t[:hybrid] (untested).
+  ~t[:incremental] uses a dpll-like algorithm to search
+  for counterexamples.
   By default this parameter is set to the symbol <tt>:simple</tt>.
-   <code>
+   ~bv[]
     Usage:
     (acl2s-defaults :set search-strategy :simple)
     (acl2s-defaults :get search-strategy)
-    :xdoc search-strategy
-   </code>
+    :doc search-strategy
+   ~ev[]
    "
  :guard (member-eq value '(:simple :incremental :hybrid)))
 ;; Use natural seeds or random tree of natural numbers 
 
 (add-acl2s-parameter 
  sampling-method :random
- :parents (ACL2::TESTING)
- :short "Specify the sampling method to be used to instantiate variables" 
- :long "Specify which of the following methods to
+ :doc-string 
+ ":Doc-Section ACL2::TESTING
+ 
+  Specify sampling method to be used to instantiate variables ~/~/
+ 
+  Specify which of the following methods to
   use for instantiating free variables of the conjecture
-  under test: <tt>:be</tt> or <tt>:random</tt> or <tt>:mixed</tt>.
-  By default this parameter is set to the symbol <tt>:random</tt>.
-   <code>
+  under test: ~t[:be] or ~t[:random] or ~t[:mixed]
+  By default this parameter is set to the symbol ~t[:random]
+   ~bv[]
     Usage:
     (acl2s-defaults :set sampling-method :random)
     (acl2s-defaults :get sampling-method)
-    :xdoc sampling-method
-   </code>
+    :doc sampling-method
+   ~ev[]
    "
  :guard (member-eq value '(:be :random :mixed)))
 
 ;; (add-acl2s-parameter 
 ;;  flatten-defdata nil
-;;  :parents (ACL2::TESTING)
-;;  :short "Flatten defdata instances during sampling"
-;;  :long "Flatten defdata enumerator expressions which stand for
+;;  :doc-string ":Doc-Section ACL2::TESTING
+;;  Flatten defdata instances during sampling"
+;;  Flatten defdata enumerator expressions which stand for
 ;;    instances of the particular defdata type. Basically if you
 ;;    have a type triple <tt>(defdata triple (list pos pos pos))</tt>,
 ;;    then an instance of triple is generated (sampled) by a call to the 
@@ -256,67 +294,77 @@ for counterexamples.
 ;;    i.e. a field of a particular type has the same distribution, 
 ;;    regardless of its position in the body of a complex defdata type.
 ;;    By default the value of parameter is <tt>nil</tt>.
-;;    <code>
+;;    ~bv[]
 ;;     Usage:
 ;;     (acl2s-defaults :set flatten-defdata-instance nil)
 ;;     (acl2s-defaults :get flatten-defdata-instance)
 ;;     :doc flatten-defdata-instance
-;;    </code>
+;;    ~ev[]
 ;;    "
 ;;  :guard (booleanp value))
 
 (add-acl2s-parameter 
  backtrack-limit 3
- :parents (ACL2::TESTING)
- :short "Maximum number of backtracks allowed (per variable)"
- :long "Maximum number of backtracks allowed by a variable.
+ :doc-string 
+ ":Doc-Section ACL2::TESTING
+ 
+  Maximum number of backtracks allowed (per variable)~/~/
+ 
+  Maximum number of backtracks allowed by a variable.
    The default backtrack limit is set to 3. Setting this 
    parameter to 0, means that backtracking is disabled.
-   <code>
+   ~bv[]
     Usage:
     (acl2s-defaults :set backtrack-limit 3)
     (acl2s-defaults :get backtrack-limit)
-    :xdoc backtrack-limit
-   </code>
+    :doc backtrack-limit
+   ~ev[]
    "
  :guard (natp value))
         
 
 (add-acl2s-parameter 
  subgoal-timeout 10
- :parents (ACL2::TESTING)
- :short "Testing timeout (in seconds) per subgoal"
- :long "Maximum allowed time (in seconds) to test any 
-   subgoal or top-level form.
-   The default timeout limit is set to 10 sec.
-   Setting this parameter to 0 amounts to disabling
-   the timeout mechanism, i.e. its a no-op.
-   <code>
+ :doc-string 
+ ":Doc-Section ACL2::TESTING
+ 
+  Testing timeout (in seconds) per subgoal~/~/
+ 
+  Maximum allowed time (in seconds) to test any 
+  subgoal or top-level form.
+  The default timeout limit is set to 10 sec.
+  Setting this parameter to 0 amounts to disabling
+  the timeout mechanism, i.e. its a no-op.
+   ~bv[]
     Usage:
     (acl2s-defaults :set subgoal-timeout 10)
     (acl2s-defaults :get subgoal-timeout)
-    :xdoc subgoal-timeout
-   </code>
+    :doc subgoal-timeout
+   ~ev[]
    "
  :guard (natp value))
 
 (add-acl2s-parameter 
  testing-enabled :naive
- :parents (ACL2::TESTING)
- :short "Testing enable/disable flag"
- :long "Testing can be enabled or disabled
-   using this parameter.
-   The default value is <tt>:naive</tt>.
-   Setting this parameter to <tt>nil</tt> amounts to disabling
-   the testing mechanism. Setting this parameter
-   to <tt>:naive</tt> leads to top-level testing without any
-   theorem prover support.
-   <code>
-    Usage:
-    (acl2s-defaults :set testing-enabled :naive)
-    (acl2s-defaults :get testing-enabled)
-    :xdoc testing-enabled
-   </code>
+ :doc-string 
+ ":Doc-Section ACL2::TESTING
+ 
+  Testing enable/disable flag~/~/
+ 
+  Testing can be enabled or disabled
+  using this parameter.
+  The default value is  ~t[:naive] (unless you are in
+  the usual ACL2 Sedan session modes, where default is ~t[t]).
+  Setting this parameter to ~t[nil] amounts to disabling
+  the testing mechanism. Setting this parameter
+  to ~t[:naive] leads to top-level testing without any
+  theorem prover support.
+  ~bv[]
+   Usage:
+   (acl2s-defaults :set testing-enabled :naive)
+   (acl2s-defaults :get testing-enabled)
+   :doc testing-enabled
+  ~ev[]
    "
  :guard (member-eq value '(T NIL :naive))
  :setter set-acl2s-random-testing-enabled)
@@ -338,18 +386,19 @@ for counterexamples.
        T))
       
 
-(defxdoc get-acl2s-random-testing-hints-enabled
-  :parents (ACL2::TESTING)
-  :short "Get current setting for random-testing-hints-enabled"
-  :long "Get current setting for random-testing-hints-enabled.
-   Returns <tt>nil</tt> if random testing is disabled 
-   i.e  thm and defthm do not make use of random-testing
-   in their proof attempts, and <tt>t</tt> otherwise.
+(defdoc get-acl2s-random-testing-hints-enabled
+  ":Doc-Section ACL2::TESTING
+  
+   Get current setting for random-testing-hints-enabled~/~/
+  
+   Get current setting for random-testing-hints-enabled.
+   Returns ~t[nil] if ~t[thm] and ~t[defthm] do not make use of random-testing
+   in their proof attempts, and ~t[t] otherwise.
    
-   <code>
+   ~bv[]
     Usage:
     (get-acl2s-random-testing-hints-enabled)
-   </code>
+   ~ev[]
    ")
 
 ;top-level exported macro to know wether random testing is enabled or not
@@ -386,26 +435,25 @@ for counterexamples.
 ;if testing-hint is disabled and user wants to turn it off its no-op
       '(value-triple :REDUNDANT)))))
 
-(defxdoc set-acl2s-random-testing-enabled
-  :parents (ACL2::TESTING)
-  :short "Control enabling/disabling random-testing"
-  :long "Control enabling/disabling random-testing.
-   By default this parameter is set to ~c[t], except in the
-   Compatible Mode.
-   If set to <tt>nil</tt>, thm and defthm retain their default ACL2 behavior.
-   If set to <tt>t</tt>, then all theorem-proving (defthm, thm, function
+(defdoc set-acl2s-random-testing-enabled
+   ":Doc-Section ACL2::TESTING
+  
+   Control enabling/disabling testing hint~/~/
+  
+   Control enabling/disabling random-testing computed override-hint.
+   If set to ~t[nil], thm and defthm retain their default ACL2 behavior.
+   If set to ~t[t], then all theorem-proving (defthm, thm, function
    termination, guard-verification) will use random-testing pervasively.
    
-   <code>
+   ~bv[]
     Usage:
     (set-acl2s-random-testing-enabled nil)
-   </code>" )
+   ~ev[]" )
+
 ;top-level exported macro to know enable random testing
 (defmacro set-acl2s-random-testing-enabled (v forms)
   (declare (xargs :guard (member-eq v '(T NIL :naive))))
-  `(with-output
-    :on :all
-    (make-event
+  `(make-event
      (let ((mode (cdr (assoc-eq :defun-mode 
                                 (table-alist
                                  'acl2::acl2-defaults-table 
@@ -413,7 +461,7 @@ for counterexamples.
        (let ((forms ',forms))
          (value `(progn
                    ,(set-acl2s-random-testing-flag-fn ,v mode state)
-                   ,@forms)))))))
+                   ,@forms))))))
 
 (defmacro acl2s-defaults (&rest rst)
   (b* (((unless (consp (cdr rst)));atleast 2 elems
@@ -438,7 +486,7 @@ for counterexamples.
                      "~|Parameter ~x0 not found in acl2s-defaults!~%"
                      ',param))
               (r (cdr param-rec-pair))
-              (val (mget :value r)))
+              (val (access acl2s-param-info% r :value)))
           val)
 
 ;get the guard and value at the runtime
@@ -457,8 +505,8 @@ for counterexamples.
                      ',param))
 ;guard is fixed once it is initialized INVARIANT
              (r (cdr param-rec-pair))
-             (guard (mget :guard r)) 
-             (setter (mget :setter r))
+             (guard (access acl2s-param-info% r :guard))
+             (setter (access acl2s-param-info% r :setter))
              (v (third ',rst)))
         `(make-event ;state changing event 
            (if (not ,(subst v 'value guard))
@@ -468,7 +516,8 @@ for counterexamples.
              (if ',setter
                  (let ((table-update-form
                         `(table acl2s-defaults-table 
-                                  ',',',param ',(c ',r :value ',v))))
+                                  ',',',param 
+                                  ',(change acl2s-param-info% ',r :value ',v))))
 ;;; setter is a macro, so dont quote the args to it whereas the above
 ;;; table macro needs quoted args because its 3rd parameter is &rest rst
                   (value `(,',setter ,',v (,table-update-form));embedded event
@@ -476,7 +525,8 @@ for counterexamples.
                            
              (value `(progn
                       (table acl2s-defaults-table 
-                             ',',',param ',(c ',r :value ',v))
+                             ',',',param 
+                             ',(change acl2s-param-info% ',r :value ',v))
                       (value-triple ',',v))))))))))))
 
 
@@ -561,6 +611,12 @@ for counterexamples.
                 acl2::keyword-alist)))))
 
 
+
+; Internal flags
+(add-acl2s-parameter 
+;show pts at the end of subgoal?
+  acl2s-pts-subgoalp NIL
+ :guard (booleanp value))
 
 
 #|ACL2s-ToDo-Line|#
