books/countereg-gen/graph.lisp
@@ -1,6 +1,6 @@
 #|$ACL2s-Preamble$;
 (ld ;; Newline to fool ACL2/cert.pl dependency scanner
- "cert.acl2")
+ "portcullis.lsp")
 (acl2::begin-book);$ACL2s-Preamble$|#
 
 ;Author: harshrc
